Use wellformedness instead of covers judgement

proof/Simple/Exp.v
@@ -3,18 +3,14 @@ Require Export Base.
 Require Export Env.
 
 
-(** Types *************************************************)
+(** Types ***********************************************************)
 Inductive ty  : Type :=
  | TCon  : nat -> ty
  | TFun  : ty  -> ty -> ty.
 Hint Constructors ty.
 
 
-(** Type Environments *************************************)
-Definition tyenv := env ty.
-
-
-(** Expressions *******************************************)
+(** Expressions *****************************************************)
 Inductive exp : Type :=
  | XVar  : nat -> exp
  | XLam  : ty  -> exp -> exp
@@ -22,43 +18,24 @@ Inductive exp : Type :=
 Hint Constructors exp.
 
 
-(** Closedness ********************************************)
-
-(* Expression is closed under an environment of a given length *)
-Inductive coversX : nat -> exp -> Prop :=
- | CoversX_var
-   :  forall n i
-   ,  (n > i) 
-   -> coversX n (XVar i)
-
- | CoversX_lam
-   :  forall n T t
-   ,  coversX (S n) t 
-   -> coversX n (XLam T t)
-
- | CoversX_app
-   :  forall n t1 t2
-   ,  coversX n t1
-   -> coversX n t2
-   -> coversX n (XApp t1 t2).
-Hint Constructors coversX.
+(** Environments ****************************************************)
+Definition tyenv := env ty.
 
 
-(* Expression is closed under the given environment. *)
-Inductive closedUnderX : tyenv -> exp -> Prop :=
- | ClosedUnderX 
-   : forall tenv x 
-   , coversX (length tenv) x -> closedUnderX tenv x. 
-Hint Constructors closedUnderX.
+(** Well Formedness *************************************************)
+
+(* Well formed expressions are closed under the given environment *)
+Fixpoint wfX (tenv: tyenv) (xx: exp) : Prop :=
+ match xx with 
+ | XVar i     => exists t, get tenv i = Some t
+ | XLam t x   => wfX (tenv :> t) x
+ | XApp x1 x2 => wfX tenv x1 /\ wfX tenv x2
+ end.
 
 
-(* Expression is closed under an empty environment, 
-   it has no free locally bound varirables *)
-Inductive closedX : exp -> Prop :=
- | ClosedX 
-   : forall xx
-   , coversX 0 xx -> closedX xx.
-Hint Constructors closedX.
+(* Closed expressions are well formed under an empty environment *)
+Definition closedX (xx: exp) : Prop
+ := wfX Empty xx.
 
 
 (* Values are closed expressions that cannot be reduced further. *)
@@ -67,18 +44,4 @@ Inductive value : exp -> Prop :=
    : forall T t
    , closedX (XLam T t) -> value (XLam T t).
 Hint Constructors value.
-
-
-(** Lemmas **********************************************************)
-Lemma closed_app
- :  forall t1 t2
- ,  closedX (XApp t1 t2) 
- -> closedX t1 /\ closedX t2.
-Proof.
- intros.
- inversions H. inversions H0.
- apply ClosedX in H3.
- apply ClosedX in H4.
- auto.
-Qed.
 
