proof/Simple/SubstValueValue.v
@@ -1,6 +1,96 @@
 
 Require Import TyJudge.
-Require Import Substitute.
+Require Export Exp.
+
+
+(** Substitution ******************************************)
+Fixpoint liftX (n: nat) (depth: nat) (tt: exp) : exp :=
+ match tt with 
+ | XVar ix    => if bge_nat ix depth
+                  then XVar (ix + n)
+                  else tt
+
+ | XLam T1 t1 => XLam T1 (liftX n (S depth) t1)
+
+ | XApp t1 t2 => XApp (liftX n depth t1)
+                      (liftX n depth t2)
+ end.
+
+
+Fixpoint subst' (depth: nat) (u: exp) (tt: exp)  : exp :=
+ match tt with
+ | XVar ix    =>  match compare ix depth with
+                  | EQ => liftX depth 0 u
+                  | GT => XVar (ix - 1)
+                  | _  => XVar ix
+                  end
+
+ | XLam T1 t2 => XLam T1 (subst' (S depth) u t2)
+
+ | XApp t1 t2 => XApp (subst' depth u t1)
+                      (subst' depth u t2)
+ end. 
+
+Definition  subst := subst' 0.
+Hint Unfold subst.
+
+
+(** Lemmas **********************************************************)
+
+(* Lifting an expression by 0 steps doesn't do anything *)
+Theorem liftX_none
+ : forall t1 depth
+ , liftX 0 depth t1 = t1.
+Proof.
+ induction t1; intro; simpl.
+
+ Case "XVar".
+  assert (n + 0 = n). omega. rewrite H.
+  breaka (bge_nat n depth).
+
+ Case "XLam".
+  rewrite IHt1. auto.
+
+ Case "XApp". 
+  rewrite IHt1_1. rewrite IHt1_2. auto.
+Qed.
+
+
+Theorem liftX_wfX
+ :  forall ix n x tenv
+ ,  n = length tenv
+ -> wfX tenv x -> liftX ix n x = x.
+Proof.
+ intros. gen tenv n.
+ induction x; intros.
+ 
+ Case "XVar".
+  simpl. breaka (bge_nat n n0).
+  simpl in H0. apply bge_nat_true in HeqX.
+  false. subst. destruct H0.
+  eapply get_above_false in H; auto.
+
+ Case "XLam".
+  simpl. simpl in H0.
+  eapply IHx in H0; eauto.
+  simpl in H0. symmetry. rewrite H. rewrite H0. auto.
+
+ Case "XApp".
+  simpl. simpl in H0. destruct H0.
+  lets D1: IHx1 H0 H. rewrite D1.
+  lets D2: IHx2 H1 H. rewrite D2.
+  auto.
+Qed.
+
+
+(* If a term is closed then lifting it doesn't do anything *)
+Theorem liftX_closed
+ : forall ix t
+ , closedX t -> liftX ix 0 t = t.
+Proof.
+ intros. unfold closedX in H. eapply liftX_wfX; eauto. 
+ simpl. auto.
+Qed.
 
 
 Theorem subst_value_value_drop
@@ -9,18 +99,18 @@ Theorem subst_value_value_drop
  -> closedX t2
  -> TYPE tenv           t1 T1
  -> TYPE (drop ix tenv) t2 T2
- -> TYPE (drop ix tenv) (subLocalX' ix t2 t1) T1.
+ -> TYPE (drop ix tenv) (subst' ix t2 t1) T1.
 Proof.
  intros ix tenv t1 t2 T1 T2. gen ix tenv T1.
  induction t1; intros.
 
  Case "XVar".
-  unfold subLocalX'.
+  unfold subst'.
   break (compare n ix).
   SCase "n = ix".
    apply compare_eq in HeqX. subst.
-   rewrite liftX_closed; auto.
-   inversions H1. rewrite H in H5. inversions H5. auto.
+   rewrite liftX_closed; eauto.
+   inverts H1. rewrite H in H5. inverts H5. auto.
 
   SCase "n < ix".
    apply compare_lt in HeqX.
@@ -55,7 +145,7 @@ Theorem subst_value_value
  ,  closedX t2
  -> TYPE (tenv :> T2) t1 T1
  -> TYPE tenv         t2 T2 
- -> TYPE tenv (subLocalX t2 t1) T1.
+ -> TYPE tenv (subst t2 t1) T1.
 Proof. 
  intros tenv t1 t2 T1 T2 Ht1 Ht2.
  lets H: subst_value_value_drop 0 (tenv :> T2).
